\documentclass{article}
\usepackage{amsmath}
\title{Scribble}
\author{Agsty}
\date{2026--02--05}
\begin{document}
\maketitle
The scribble is as follows:
\[
    \int
    _{\frac{\lim_{u\to\infty}(1+\frac{1}{u})^u}
    {\lim_{u\to\infty}(\frac{e^u+2u^2-1}{4u^4-1})}}
    ^{\int_0^{\ln(\frac{4!-\sqrt{9}}{(2!)^{2!+2!}})^{-1}}\int_0^1\frac{2w^2-4w-16}{w^3-64}dw\ dy}
    \sum_{k=1}^{\infty}((\lim_{n\to\infty}\int_1^n\frac{\tan\frac{3\pi}{4}}{x^2}dx)^k(\frac{d}{dx}\int_{68!}^{x}t\ dt)^{2k})dx
\]
Evaluating the lower limit, starting with the numerator:
\[
\lim_{u\to\infty}(1+\frac{1}{u})^u=e
\]
The denominator:
\[
\lim_{u\to\infty}(\frac{e^u+2u^2-1}{4u^4-1})
\]
Using L'Hopital's Rule:
\[
f(u) = e^u + 2u^2 -1,\ g(u) = 4u^4 - 1
\]
1st derivatives:
\[
f'(u) = e^u + 4u,\ g'(u) = 16u^3
\]
2nd derivatives:
\[
f''(u) = e^u + 4,\ g''(u) = 48u^2
\]
3rd derivatives:
\[
f^{(3)}(u) = e^u,\ g^{(3)}(u) = 96u
\]
4th derivatives:
\[
f^{(4)}(u) = e^u,\ g^{(4)}(u) = 96
\]
Evaluating the limit:
\[
\lim_{u\to\infty}(\frac{e^u}{96}) = \infty
\]
Fully evaluating the lower limit:
\[
\frac{\lim_{u\to\infty}(1+\frac{1}{u})^u}
{\lim_{u\to\infty}(\frac{e^u+2u^2-1}{4u^4-1})}
= \frac{e}{\infty} = 0
\]
Rewriting the integral:
\[
    \int
    _0
    ^{\int_0^{\ln(\frac{4!-\sqrt{9}}{(2!)^{2!+2!}})^{-1}}\int_0^1\frac{2w^2-4w-16}{w^3-64}dw\ dy}
    \sum_{k=1}^{\infty}((\lim_{n\to\infty}\int_1^n\frac{\tan\frac{3\pi}{4}}{x^2}dx)^k(\frac{d}{dx}\int_{68!}^{x}t\ dt)^{2k})dx
\]
Evaluating the upper limit:
\[
\int_0^{\ln(\frac{4!-\sqrt{9}}{(2!)^{2!+2!}})^{-1}}\int_0^1\frac{2w^2-4w-16}{w^3-64}dw\ dy
\]
Evaluate the logarithm in the upper limit of the first integral:
\[
\ln(\frac{4!-\sqrt{9}}{(2!)^{2!+2!}})^{-1}=\ln(\frac{24-3}{2^{2+2}})^{-1}=\ln(\frac{21}{16})^{-1}
\]
Rewriting:
\[
\int_0^{\ln(\frac{21}{16})^{-1}}\int_0^1\frac{2w^2-4w-16}{w^3-64}dw\ dy
\]
Simplifying the integrand:
\[
\frac{2w^2-4w-16}{w^3-64}=\frac{(w-4)(2w+4)}{(w-4)(w^2+4w+16)}=\frac{2w+4}{w^2+4w+16}
\]
Using a u-substitution:
\[
u = w^2+4w+16,\ \frac{du}{dw} = 2w + 4,\ du=(2w+4)dw
\]
Modifying the limits:
\[
@w=1,\ u=1+4+16=21,\ @w=0,\ u=0+0+16=16
\]
Rewriting the inner integral:
\[
\int_{16}^{21}\frac{1}{u}du
\]
Integrating:
\[
[\ln|u|]^{21}_{16} = \ln(21)-\ln(16) = \ln(\frac{21}{16})
\]
The outer integral:
\[
\int_0^{\ln(\frac{21}{16})^{-1}}\ln(\frac{21}{16})dy
\]
Integrate and evaluate:
\[
[y\ln(\frac{21}{16})]^{\ln(\frac{21}{16})^{-1}}_0 = \ln(\frac{21}{16})\ln(\frac{21}{16})^{-1} - 0 = 1-0 = 1
\]
Rewriting the entire integral:
\[
    \int
    _0^1
    \sum_{k=1}^{\infty}((\lim_{n\to\infty}\int_1^n\frac{\tan\frac{3\pi}{4}}{x^2}dx)^k(\frac{d}{dx}\int_{68!}^{x}t\ dt)^{2k})dx
\]
Evaluating the first part of the sum:
\[
(\lim_{n\to\infty}\int_1^n\frac{\tan\frac{3\pi}{4}}{x^2}dx)^k
\]
Simplify the integrand:
\[
\tan\frac{3\pi}{4}=-1,\ \frac{1}{x^2}=x^{-2}
\]
\[
(\lim_{n\to\infty}\int_1^n -x^{-2}dx)^k
\]
Integrate and evaluate:
\[
[\frac{1}{x}]^{\infty}_{1} = \frac{1}{\infty} - 1 = 0 - 1 = -1
\]
Therefore this part of the sum is:
\[
(-1)^k
\]
Rewriting the full integral:
\[
    \int
    _0^1
    \sum_{k=1}^{\infty}((-1)^k(\frac{d}{dx}\int_{68!}^{x}t\ dt)^{2k})dx
\]
Evaluate the second part of the sum:
\[
(\frac{d}{dx}\int_{68!}^{x}t\ dt)^{2k}
\]
Using the Fundamental Theorem of Calculus:
\[
\text{If }f\in([a,b]),\ \text{then } \frac{d}{dx}\int_a^x f(t)dt=f(x)
\]
Therefore:
\[
(\frac{d}{dx}\int_{68!}^{x}t\ dt)^{2k}=x^{2k}
\]
Rewriting the full integral:
\[
    \int
    _0^1
    \sum_{k=1}^{\infty}((-1)^k x^{2k})dx
\]
Evalutating the sum:
\[
\sum_{k=1}^{\infty}((-1)^k x^{2k})=\sum_{k=1}^{\infty}(-1)^k(x^2)^k=\sum_{k=1}^{\infty}(-x^2)^k
\]
Using the infinite summation formula:
\[
\sum_{k=1}^{\infty}(r^k)=\frac{r}{1-r},\ |r|<1
\]
Therefore:
\[
|-x^2|<1,\ x^2<1,\ x<1
\]
As the integral is over $x\in [0,1]$, converges for $x\in [0,1)$, and the integral when $x=1$ 
has width $0$, so doesn't affect the integral, we can use the infinite summation formula. Therefore, the integral rewrites as:
\[
\int_0^1\frac{-x^2}{1+x^2}dx
\]
Pulling out the minus sign and breaking down the factors:
\[
\int_0^1-\frac{1+x^2-1}{1+x^2}dx=
-(\int_0^1\frac{1+x^2}{1+x^2}-\frac{1}{1+x^2}dx)=
-(\int_0^1 1 dx - \int_0^1 \frac{1}{1+x^2}dx )
\]
Multiplying throughout by -1:
\[
\int_0^1\frac{1}{1+x^2}dx - \int_0^1 1dx
\]
Integrating:
\[
[\arctan(x)-x]_0^1
\]
Evaluate:
\[
[(\arctan(1)-1)-(\arctan(0)-0)] = [(\frac{\pi}{4}-1)-(0-0)]=\frac{\pi}{4}-1
\]
\end{document}
